LLVM_DS_RBT/Lookup/Lookup.thy
@@ -2,6 +2,8 @@ theory Lookup
   imports 
     "../Setup"
     "../Bool_Assn_Setup"
+    "../Utilities"
+    Rbt_Pointer
     OptionI
 begin
 
@@ -37,9 +39,9 @@ definition "rbt_contains t k \<equiv> rbt_lookup t k \<noteq> None"
 
 lemma contains_correct:
   "llvm_htriple
-  (\<upharpoonleft>rbt_assn t ti ** \<upharpoonleft>key_assn k ki)
+  (rbt_assn t ti ** \<upharpoonleft>key_assn k ki)
   (contains ti ki)
-  (\<lambda>ri. \<upharpoonleft>bool.assn (rbt_contains t k) ri ** \<upharpoonleft>rbt_assn t ti ** \<upharpoonleft>key_assn k ki)"
+  (\<lambda>ri. \<upharpoonleft>bool.assn (rbt_contains t k) ri ** rbt_assn t ti ** \<upharpoonleft>key_assn k ki)"
 proof(induction t arbitrary: ti)
   case Empty
   then show ?case
@@ -50,7 +52,7 @@ proof(induction t arbitrary: ti)
 next
   case (Branch c lhs key val rhs)
   note [vcg_rules] = Branch.IH
-  note [simp] = rbt_contains_def rbt_assn_branch_def
+  note [simp] = rbt_contains_def
 
   show ?case
     apply (subst contains.simps)
@@ -74,8 +76,8 @@ abbreviation "alloc_opt_none \<equiv> do {
 
 
 partial_function (M) lookup ::
-  "('ki, 'vi) rbti \<Rightarrow> 'ki \<Rightarrow> 'vi option_i llM" where
-  "lookup node_p k = do {
+  "('vi \<Rightarrow> 'vi llM) \<Rightarrow> ('ki, 'vi) rbti \<Rightarrow> 'ki \<Rightarrow> 'vi option_i llM" where
+  "lookup value_copy node_p k = do {
     if node_p = null
     then return (OPTION_I init 0)
     else do {
@@ -83,11 +85,11 @@ partial_function (M) lookup ::
       k_old \<leftarrow> return rbt_node.key node;
       k_lt \<leftarrow> lt_impl k k_old;
       if k_lt = 1
-      then lookup (rbt_node.left node) k
+      then lookup value_copy (rbt_node.left node) k
       else do {
         k_gt \<leftarrow> lt_impl k_old k;
         if k_gt = 1
-        then lookup (rbt_node.right node) k
+        then lookup value_copy (rbt_node.right node) k
         else do {
           val_copy \<leftarrow> value_copy (rbt_node.val node);
           return (OPTION_I val_copy 1)
@@ -107,13 +109,24 @@ definition "value_option_assn \<equiv> v_option.option_assn"
 
 
 lemma lookup_correct [vcg_rules]:
-  "llvm_htriple
-  (\<upharpoonleft>rbt_assn t ti ** \<upharpoonleft>key_assn k ki)
-  (lookup ti ki)
-  (\<lambda>opt.
-    \<upharpoonleft>value_option_assn (rbt_lookup t k) opt **
-    \<upharpoonleft>rbt_assn t ti **
-    \<upharpoonleft>key_assn k ki)"
+  assumes
+    copy_rule [vcg_rules]:
+    "\<And>v vi.
+      llvm_htriple
+      (\<upharpoonleft>value_assn v vi)
+      (value_copy vi)
+      (\<lambda>r. \<upharpoonleft>value_assn v vi ** \<upharpoonleft>value_assn v r)
+    "   
+  shows
+    "
+      llvm_htriple
+      (rbt_assn t ti ** \<upharpoonleft>key_assn kn ki)
+      (lookup value_copy ti ki)
+      (\<lambda>opt.
+        \<upharpoonleft>value_option_assn (rbt_lookup t kn) opt **
+        rbt_assn t ti **
+        \<upharpoonleft>key_assn kn ki)
+    "
 proof(induction t arbitrary: ti)
   case Empty
   then show ?case
@@ -122,12 +135,11 @@ proof(induction t arbitrary: ti)
     apply vcg
     done
 next
-  case (Branch x1 t1 x3 x4 t2)
+  case (Branch c l k v r)
 
   note [vcg_rules] = Branch.IH
-  note [simp] = rbt_assn_branch_def
 
-  show ?case
+  from Branch show ?case
     apply (subst lookup.simps)
     apply vcg
     unfolding value_option_assn_def
@@ -137,13 +149,25 @@ qed
 
 
 lemma lookup_correct_mem [vcg_rules]:
-  "llvm_htriple
-  (rbt_assn_mem t ptrs ti ** \<upharpoonleft>key_assn k ki)
-  (lookup ti ki)
-  (\<lambda>opt.
-    \<upharpoonleft>value_option_assn (rbt_lookup t k) opt **
-    rbt_assn_mem t ptrs ti **
-    \<upharpoonleft>key_assn k ki)"
+  assumes
+    copy_rule [vcg_rules]:
+    "\<And>v vi.
+      llvm_htriple
+      (\<upharpoonleft>value_assn v vi)
+      (value_copy vi)
+      (\<lambda>r. \<upharpoonleft>value_assn v vi ** \<upharpoonleft>value_assn v r)
+    " and
+    "k \<notin> ex"
+  shows
+    "
+      llvm_htriple
+      (rbt_assn_cplx t ptrs ex ti ** \<upharpoonleft>key_assn k ki)
+      (lookup value_copy ti ki)
+      (\<lambda>opt.
+        \<upharpoonleft>value_option_assn (rbt_lookup t k) opt **
+        rbt_assn_cplx t ptrs ex ti **
+        \<upharpoonleft>key_assn k ki)
+    "
 proof(induction t arbitrary: ti)
   case Empty
   then show ?case
@@ -152,18 +176,271 @@ proof(induction t arbitrary: ti)
     apply vcg
     done
 next
-  case (Branch x1 t1 x3 x4 t2)
+  case Branch
 
   note [vcg_rules] = Branch.IH
-  note [simp] = rbt_assn_branch_def
 
   show ?case
     apply (subst lookup.simps)
     apply vcg
+    apply (simp add: `k\<notin>ex`)
     unfolding value_option_assn_def
     apply vcg
     done
 qed
+
+
+partial_function (M) lookup_ptr ::
+  "('ki, 'vi) rbti \<Rightarrow> 'ki \<Rightarrow> ('ki, 'vi) rbti llM" where
+  "lookup_ptr node_p k = do {
+    if node_p = null
+    then return null
+    else do {
+      node \<leftarrow> ll_load node_p;
+      k_old \<leftarrow> return rbt_node.key node;
+      if! lt_impl k k_old
+      then! lookup_ptr (rbt_node.left node) k
+      else! if! lt_impl k_old k
+      then! lookup_ptr (rbt_node.right node) k
+      else! return node_p
+    }
+  }"
+
+
+lemma lookup_ptr_rule [vcg_rules]:
+  "
+    rbt_sorted t \<Longrightarrow>
+    llvm_htriple
+    (rbt_assn_cplx t ptrs ex ti ** \<upharpoonleft>key_assn kn ki)
+    (lookup_ptr ti ki)
+    (\<lambda>ptr. rbt_assn_cplx t ptrs ex ti ** \<upharpoonleft>key_assn kn ki **
+      \<up>(if ptr = null then kn \<notin> rbt_key_set t else ptr = fst (the (ptrs kn)) \<and> kn \<in> rbt_key_set t ))
+  "
+proof(induction t arbitrary: ti)
+  case Empty
+  then show ?case 
+    apply(subst lookup_ptr.simps)
+    apply vcg
+    done
+next
+  case (Branch c l k v r)
+  
+  note Branch[vcg_rules]
+
+  from Branch(3) show ?case
+    apply(subst lookup_ptr.simps)
+    apply vcg
+    subgoal
+      apply vcg_compat
+      apply isep_solver
+      unfolding rbt_greater_prop apply auto
+      done
+
+    apply vcg
+    subgoal
+      apply vcg_compat
+      apply isep_solver
+      unfolding rbt_less_prop apply auto
+      done
+
+    apply vcg
+    done
+qed
+
+
+definition lookup_ptr_to_option where
+  "lookup_ptr_to_option value_copy t k \<equiv>
+    do {
+      res_p \<leftarrow> lookup_ptr t k;
+      if res_p = null
+      then return (OPTION_I init 0)
+      else do {
+        v \<leftarrow> rbt_ptr_load res_p;
+        v_copy \<leftarrow> value_copy v;
+        return (OPTION_I v_copy 1)
+      }
+    }
+  "
+
+
+lemma H: 
+  "(\<And>x. llvm_htriple (P x) C (\<lambda>r. Q x r)) \<Longrightarrow>
+  llvm_htriple (EXS x. P x) C (\<lambda>r. EXS x. Q x r) "
+  unfolding htriple_def wpa_def STATE_def NEMonad.wp_def Sep_Generic_Wp.wp_def
+  by blast
+
+
+(*
+lemma lookup_ptr_rule':
+"
+    rbt_sorted t \<Longrightarrow>
+    llvm_htriple
+    (EXS ptrs ex. rbt_assn_cplx t ptrs ex ti ** \<upharpoonleft>key_assn kn ki)
+    (lookup_ptr ti ki)
+    (\<lambda>ptr. EXS ptrs ex. rbt_assn_cplx t ptrs ex ti ** \<upharpoonleft>key_assn kn ki ** \<up>(if ptr = null then kn \<notin> rbt_key_set t else ptr = the (ptrs kn)))
+"
+  apply (rule H)+
+  apply (rule lookup_ptr_rule)
+  apply assumption
+  done
+*)
+
+
+lemma rbt_lookup_none_keys:
+ "rbt_sorted t \<Longrightarrow> k \<notin> rbt_key_set t \<Longrightarrow> rbt_lookup t k = None"
+  using rbt_lookup_iff_keys
+  by blast
+
+
+lemma rbt_lookup_some_keys:
+  assumes "rbt_sorted t" and "k \<in> rbt_key_set t" obtains v where "rbt_lookup t k = Some v"
+  using rbt_lookup_iff_keys assms
+  by blast
+
+find_theorems rbt_assn_cplx RBT_Impl.keys
+
+lemma rbt_assn_cplx_join:
+      "kn \<in> rbt_key_set t \<Longrightarrow> rbt_sorted t \<Longrightarrow>
+      rbt_assn_cplx t ptrs {kn} ti ** \<upharpoonleft>value_assn (the (rbt_lookup t kn)) (snd (the (ptrs kn)))
+      \<turnstile> rbt_assn_cplx t ptrs {} ti"
+proof(induction t arbitrary: ti)
+  case Empty
+  then show ?case by simp
+next
+  case (Branch c l k v r)
+
+  have H1: "(x::'a::linorder) < y \<Longrightarrow> \<not>(y < x)" for x y by simp
+
+  from Branch(3-4) show ?case
+    
+    apply (rule rbt_key_set_cases)
+
+    subgoal
+      apply simp
+      apply isep_elim_ex
+      apply isep_intro_ex
+      apply isep_solver_keep
+      apply simp
+      apply isep_solver_keep
+      done
+
+    subgoal
+      apply simp
+      apply isep_elim_ex
+      apply isep_intro_ex
+      apply (isep_drule drule: Branch(1))
+      using Branch(4) apply auto
+      apply isep_solver_keep
+      done
+
+    subgoal
+      apply (simp split del: if_split)
+      apply isep_elim_ex
+      apply isep_intro_ex
+      apply (isep_drule drule: Branch(2))
+      using Branch(4) apply (simp_all add: H1)
+      apply isep_assumption+
+      done
+
+    done
+qed
+  
+
+lemma lookup_ptr_to_option_correct_cplx [vcg_rules]:
+  assumes
+    copy_rule [vcg_rules]:
+    "\<And>v vi.
+      llvm_htriple
+      (\<upharpoonleft>value_assn v vi)
+      (value_copy vi)
+      (\<lambda>r. \<upharpoonleft>value_assn v vi ** \<upharpoonleft>value_assn v r)
+    "   
+  shows
+    "
+      rbt_sorted t \<Longrightarrow>
+      llvm_htriple
+      (rbt_assn_cplx t ptrs {} ti ** \<upharpoonleft>key_assn kn ki)
+      (lookup_ptr_to_option value_copy ti ki)
+      (\<lambda>opt.
+        \<upharpoonleft>value_option_assn (rbt_lookup t kn) opt **
+        rbt_assn_cplx t ptrs {} ti **
+        \<upharpoonleft>key_assn kn ki)
+    "
+  unfolding lookup_ptr_to_option_def
+  apply vcg
+  subgoal
+    unfolding value_option_assn_def
+    apply (simp add: rbt_lookup_none_keys)
+    apply vcg
+    done
+  apply vcg
+  subgoal
+    unfolding value_option_assn_def
+    apply vcg_compat
+    apply (rule rbt_lookup_some_keys, simp, simp)
+    apply (isep_solver_keep isep_dest: rbt_assn_cplx_join | simp)+
+    done
+  done
+
+
+lemma htriple_ent_pre_post:
+  "\<lbrakk>htriple P' c Q'; P \<turnstile> P'; \<And>r. Q' r \<turnstile> Q r\<rbrakk> \<Longrightarrow> htriple P c Q"
+  using htriple_ent_pre htriple_ent_post by blast
+
+
+lemma lookup_ptr_to_option_correct_cplx' [vcg_rules]:
+  assumes
+    copy_rule [vcg_rules]:
+    "\<And>v vi.
+      llvm_htriple
+      (\<upharpoonleft>value_assn v vi)
+      (value_copy vi)
+      (\<lambda>r. \<upharpoonleft>value_assn v vi ** \<upharpoonleft>value_assn v r)
+    "   
+  shows
+    "
+      rbt_sorted t \<Longrightarrow>
+      llvm_htriple
+      (EXS ptrs. rbt_assn_cplx t ptrs {} ti ** \<upharpoonleft>key_assn kn ki)
+      (lookup_ptr_to_option value_copy ti ki)
+      (\<lambda>opt. EXS ptrs.
+        \<upharpoonleft>value_option_assn (rbt_lookup t kn) opt **
+        rbt_assn_cplx t ptrs {} ti **
+        \<upharpoonleft>key_assn kn ki)
+    "
+  apply (rule H)
+  using copy_rule lookup_ptr_to_option_correct_cplx by simp
+
+
+lemma lookup_ptr_to_option_correct [vcg_rules]:
+  assumes
+    copy_rule [vcg_rules]:
+    "\<And>v vi.
+      llvm_htriple
+      (\<upharpoonleft>value_assn v vi)
+      (value_copy vi)
+      (\<lambda>r. \<upharpoonleft>value_assn v vi ** \<upharpoonleft>value_assn v r)
+    "   
+  shows
+    "
+      rbt_sorted t \<Longrightarrow>
+      llvm_htriple
+      (rbt_assn t ti ** \<upharpoonleft>key_assn kn ki)
+      (lookup_ptr_to_option value_copy ti ki)
+      (\<lambda>opt.
+        \<upharpoonleft>value_option_assn (rbt_lookup t kn) opt **
+        rbt_assn t ti **
+        \<upharpoonleft>key_assn kn ki)
+    "
+  using lookup_ptr_to_option_correct_cplx
+  apply - 
+  apply (rule htriple_ent_pre_post[OF lookup_ptr_to_option_correct_cplx'])
+  using copy_rule apply simp
+    apply simp
+   apply (isep_solver_keep isep_dest: rbt_assn_entails_rbt_assn_cplx)
+   apply simp
+  apply (isep_solver_keep isep_dest: rbt_assn_cplx_entails_rbt_assn)
+  done
 
 
 end
