LLVM_DS_RBT/Delete/Combine.thy
@@ -72,9 +72,9 @@ partial_function (M) combine ::
 lemma combine_correct [vcg_rules]:
   "
   llvm_htriple
-  (\<upharpoonleft>rbt_assn l li ** \<upharpoonleft>rbt_assn r ri)
+  (rbt_assn l li ** rbt_assn r ri)
   (combine li ri)
-  (\<lambda>x. \<upharpoonleft>rbt_assn (rbt_combine l r) x)
+  (\<lambda>x. rbt_assn (rbt_combine l r) x)
 "
 proof(induction l r arbitrary: li ri rule: RBT_Impl.combine.induct)
   case (1 x)
