LLVM_DS_RBT/Lookup/Rbt_Pointer.thy
@@ -1,0 +1,123 @@
+theory Rbt_Pointer
+  imports Setup
+begin
+
+
+context rbt_impl
+begin
+
+
+interpretation monad_syntax_M_loc .
+
+
+definition rbt_ptr_load :: "('ki, 'vi) rbti \<Rightarrow> 'vi llM" where
+  "rbt_ptr_load p \<equiv> do { n \<leftarrow> ll_load p; return rbt_node.val n }"
+
+
+lemma pure_part_exE:
+    assumes "pure_part (\<lambda>s. \<exists>x. P x s)"
+    obtains x where "pure_part (P x)"
+  using assms unfolding pure_part_def by blast
+  
+
+lemma rbt_assn_cplx_ptrs_someI:
+  "\<lbrakk>k \<in> set (RBT_Impl.keys t); pure_part (rbt_assn_cplx t ptrs ex ti)\<rbrakk> \<Longrightarrow> 
+  \<exists>p. ptrs k = Some p"
+proof(induction t arbitrary: ti)
+  case Empty
+  then show ?case by simp
+next
+  case (Branch c k l v r)
+  then show ?case
+    apply auto
+    subgoal by (auto dest!: pure_part_split_conj elim!: pure_part_exE)
+    subgoal by (auto dest!: pure_part_split_conj elim!: pure_part_exE)
+    subgoal by (auto dest!: pure_part_split_conj elim!: pure_part_exE)
+    done
+qed
+
+
+lemma rbt_assn_cplx_ptrs_domI:
+  "\<lbrakk>pure_part (rbt_assn_cplx t ptrs ex ti)\<rbrakk> \<Longrightarrow> set (RBT_Impl.keys t) \<subseteq> dom ptrs"
+  using rbt_assn_cplx_ptrs_someI by blast  
+
+
+lemma rbt_assn_cplx_extra_ex [simp]:
+  "k \<notin> set (RBT_Impl.keys t) \<Longrightarrow> rbt_assn_cplx t ptrs (insert k ex) ti = rbt_assn_cplx t ptrs ex ti"
+  by (induction t arbitrary: ti, auto)
+
+
+lemma rbt_key_set_cases:
+  assumes
+    "kn \<in> rbt_key_set (rbt.Branch c l k v r)" and
+    "rbt_sorted (rbt.Branch c l k v r)" and
+    "\<lbrakk>kn = k; kn \<notin> rbt_key_set l; kn \<notin> rbt_key_set r\<rbrakk> \<Longrightarrow> thesis" and
+    "\<lbrakk>kn \<noteq> k; kn \<in> rbt_key_set l; kn < k; kn \<notin> rbt_key_set r\<rbrakk> \<Longrightarrow> thesis" and
+    "\<lbrakk>kn \<noteq> k; kn \<notin> rbt_key_set l; kn > k; kn \<in> rbt_key_set r\<rbrakk> \<Longrightarrow> thesis"
+  shows
+    thesis
+  using assms
+  apply (fastforce simp add: rbt_greater_prop rbt_less_prop)
+  done
+
+
+lemma rbt_ptr_load_correct' [vcg_rules]:
+  assumes
+    "rbt_sorted t" and
+    "kn \<in> rbt_key_set t" and
+    "kn \<notin> ex"
+  shows
+    "
+    llvm_htriple
+    (rbt_assn_cplx t ptrs ex ti)
+    (rbt_ptr_load (fst (the (ptrs kn))) )
+    (\<lambda>vi. \<upharpoonleft>value_assn (the (rbt_lookup t kn)) vi ** rbt_assn_cplx t ptrs (ex \<union> {kn}) ti **
+      \<up>(vi = snd (the (ptrs kn))))
+    "
+  using assms
+proof(induction t arbitrary: ti)
+  case Empty 
+  then show ?case by simp
+next
+  case (Branch c l k v r)
+  from Branch(3-5) show ?case
+    apply -
+
+    apply (rule rbt_key_set_cases, assumption, assumption)
+
+    subgoal unfolding rbt_ptr_load_def by vcg
+    subgoal
+      supply Branch(1)[vcg_rules]
+      apply vcg
+      done
+    subgoal
+      supply Branch(2)[vcg_rules]
+      apply vcg
+      apply auto (*unnecessarily splits the k \<in> ex if*)
+       apply vcg
+      done
+    done
+qed
+
+
+lemma rbt_ptr_load_correct :
+  assumes
+    "rbt_sorted t" and
+    "rbt_lookup t kn = Some v" and
+    "kn \<notin> ex"
+  shows
+    "
+    llvm_htriple
+    (rbt_assn_cplx t ptrs ex ti)
+    (rbt_ptr_load (fst (the (ptrs kn))) )
+    (\<lambda>vi. \<upharpoonleft>value_assn v vi ** rbt_assn_cplx t ptrs (ex \<union> {kn}) ti **
+      \<up>(vi = snd (the (ptrs kn))))
+    "
+  using assms rbt_ptr_load_correct' rbt_lookup_iff_keys(3)
+  by (smt (verit, del_insts) entails_eq_iff htriple_ent_post option.sel)
+
+
+end
+
+
+end
