LLVM_DS_RBT/Zipper_Iterator/Iterator.thy
@@ -1,0 +1,18 @@
+theory Iterator
+  imports 
+    Zipper
+    "../Separation_Logic_Solver/Methods"
+begin
+
+
+context rbt_impl
+begin
+interpretation llvm_prim_ctrl_setup .
+interpretation llvm_prim_arith_setup .
+interpretation llvm_prim_setup .
+
+
+end
+
+
+end
